ulib/FStar.Map.fst
@@ -1,5 +1,5 @@
 module FStar.Map
-open FStar.Set
+open FStar.BSet
 open FStar.FunctionalExtensionality
 
 noeq abstract type t (key:eqtype) (value:Type) = {
@@ -18,116 +18,113 @@ abstract val domain: #key:eqtype -> #value:Type -> t key value -> Tot (set key)
 let sel #key #value m k = m.mappings k
 let upd #key #value m k v = {
   mappings = (fun x -> if x = k then v else m.mappings x);
-  domain =   Set.union m.domain (Set.singleton k)
+  domain =   union m.domain (singleton k)
 }
 let const #key #value v = {
   mappings = (fun _ -> v);
-  domain =   Set.complement Set.empty
+  domain =   complement empty
 }
-
-val foo: nat -> Tot nat
-let foo n =
 
 let concat #key #value m1 m2 = {
-  mappings = (fun x -> if Set.mem x m2.domain then m2.mappings x else m1.mappings x);
-  domain =   Set.union m1.domain m2.domain
+  mappings = (fun x -> if mem x m2.domain then m2.mappings x else m1.mappings x);
+  domain =   union m1.domain m2.domain
 }
-let contains m k = Set.mem k m.domain
-let restrict s m = {
+let contains #key #value m k = mem k m.domain
+let restrict #key #value s m = {
   mappings = m.mappings;
-  domain =   Set.intersect s m.domain
+  domain =   intersect s m.domain
 }
-let domain m = m.domain
+let domain #key #value m = m.domain
 
-abstract val lemma_SelUpd1: m:t 'key 'value -> k:'key -> v:'value ->
-                   Lemma (requires True) (ensures (sel (upd m k v) k = v))
+abstract val lemma_SelUpd1: #key:eqtype -> #value:Type -> m:t key value -> k:key -> v:value ->
+                   Lemma (requires True) (ensures (sel (upd m k v) k == v))
 		   [SMTPat (sel (upd m k v) k)]
 
-abstract val lemma_SelUpd2: m:t 'key 'value -> k1:'key -> k2:'key -> v:'value ->
-                   Lemma (requires True) (ensures (k2=!=k1 ==> sel (upd m k2 v) k1 = sel m k1))
+abstract val lemma_SelUpd2: #key:eqtype -> #value:Type -> m:t key value -> k1:key -> k2:key -> v:value ->
+                   Lemma (requires True) (ensures (k2=!=k1 ==> sel (upd m k2 v) k1 == sel m k1))
                    [SMTPat (sel (upd m k2 v) k1)]
 
-abstract val lemma_SelConst: v:'value -> k:'key ->
+abstract val lemma_SelConst: #key:eqtype -> #value:Type -> v:value -> k:key ->
                     Lemma (requires True) (ensures (sel (const v) k == v))
                     [SMTPat (sel (const v) k)]
 
-abstract val lemma_SelRestrict: m:t 'key 'value -> ks:set 'key -> k:'key ->
+abstract val lemma_SelRestrict: #key:eqtype -> #value:Type -> m:t key value -> ks:set key -> k:key ->
                        Lemma (requires True) (ensures (mem k ks ==> sel (restrict ks m) k == sel m k))
                        [SMTPat (sel (restrict ks m) k)]
 
-abstract val lemma_SelConcat1: m1:t 'key 'value -> m2:t 'key 'value -> k:'key ->
+abstract val lemma_SelConcat1: #key:eqtype -> #value:Type -> m1:t key value -> m2:t key value -> k:key ->
                       Lemma (requires True) (ensures (contains m2 k ==> sel (concat m1 m2) k==sel m2 k))
                       [SMTPat (sel (concat m1 m2) k)]
 
-abstract val lemma_SelConcat2: m1:t 'key 'value -> m2:t 'key 'value -> k:'key ->
+abstract val lemma_SelConcat2: #key:eqtype -> #value:Type -> m1:t key value -> m2:t key value -> k:key ->
                       Lemma (requires True) (ensures (not(contains m2 k) ==> sel (concat m1 m2) k==sel m1 k))
                       [SMTPat (sel (concat m1 m2) k)]
 
-abstract val lemma_InDomUpd1: m:t 'key 'value -> k1:'key -> k2:'key -> v:'value ->
+abstract val lemma_InDomUpd1: #key:eqtype -> #value:Type -> m:t key value -> k1:key -> k2:key -> v:value ->
                      Lemma (requires True) (ensures (contains (upd m k1 v) k2 == (k1=k2 || contains m k2)))
                      [SMTPat (contains (upd m k1 v) k2)]
 
-abstract val lemma_InDomUpd2: m:t 'key 'value -> k1:'key -> k2:'key -> v:'value ->
+abstract val lemma_InDomUpd2: #key:eqtype -> #value:Type -> m:t key value -> k1:key -> k2:key -> v:value ->
                      Lemma (requires True) (ensures (k2=!=k1 ==> contains (upd m k2 v) k1 == contains m k1))
                      [SMTPat (contains (upd m k2 v) k1)]
 
-abstract val lemma_InDomConstMap: v:'value -> k:'key ->
+abstract val lemma_InDomConstMap: #key:eqtype -> #value:Type -> v:value -> k:key ->
                          Lemma (requires True) (ensures (contains (const v) k))
                          [SMTPat (contains (const v) k)]
 
-abstract val lemma_InDomConcat: m1:t 'key 'value -> m2:t 'key 'value -> k:'key ->
+abstract val lemma_InDomConcat: #key:eqtype -> #value:Type -> m1:t key value -> m2:t key value -> k:key ->
                  Lemma (requires True) (ensures (contains (concat m1 m2) k==(contains m1 k || contains m2 k)))
                  [SMTPat (contains (concat m1 m2) k)]
 
-abstract val lemma_InDomRestrict: m:t 'key 'value -> ks:set 'key -> k:'key ->
+abstract val lemma_InDomRestrict: #key:eqtype -> #value:Type -> m:t key value -> ks:set key -> k:key ->
                          Lemma (requires True) (ensures (contains (restrict ks m) k == (mem k ks && contains m k)))
                          [SMTPat (contains (restrict ks m) k)]
 
-abstract val lemma_ContainsDom: m:t 'key 'value -> k:'key -> 
-  Lemma (requires True) (ensures (contains m k = Set.mem k (domain m)))
+abstract val lemma_ContainsDom: #key:eqtype -> #value:Type -> m:t key value -> k:key -> 
+  Lemma (requires True) (ensures (contains m k = mem k (domain m)))
                       [SMTPat (contains m k)]
 
-abstract val lemma_UpdDomain : m:t 'key 'value -> k:'key -> v:'value ->
+abstract val lemma_UpdDomain : #key:eqtype -> #value:Type -> m:t key value -> k:key -> v:value ->
   Lemma (requires True) 
-	(ensures (Set.equal (domain (upd m k v)) (Set.union (domain m) (Set.singleton k))))
+	(ensures (equal (domain (upd m k v)) (union (domain m) (singleton k))))
 	[SMTPat (domain (upd m k v))]
   
-let lemma_SelUpd1 m k v        = ()
-let lemma_SelUpd2 m k1 k2 v    = ()
-let lemma_SelConst v k         = ()
-let lemma_SelRestrict m ks k   = ()
-let lemma_SelConcat1 m1 m2 k   = ()
-let lemma_SelConcat2 m1 m2 k   = ()
-let lemma_InDomUpd1 m k1 k2 v  = ()
-let lemma_InDomUpd2 m k1 k2 v  = ()
-let lemma_InDomConstMap v k    = ()
-let lemma_InDomConcat m1 m2 k  = ()
-let lemma_InDomRestrict m ks k = ()
-let lemma_ContainsDom m k      = ()
-let lemma_UpdDomain m k v      = ()
+let lemma_SelUpd1 #key #value m k v        = ()
+let lemma_SelUpd2 #key #value m k1 k2 v    = ()
+let lemma_SelConst #key #value v k         = ()
+let lemma_SelRestrict #key #value m ks k   = ()
+let lemma_SelConcat1 #key #value m1 m2 k   = ()
+let lemma_SelConcat2 #key #value m1 m2 k   = ()
+let lemma_InDomUpd1 #key #value m k1 k2 v  = ()
+let lemma_InDomUpd2 #key #value m k1 k2 v  = ()
+let lemma_InDomConstMap #key #value v k    = ()
+let lemma_InDomConcat #key #value m1 m2 k  = ()
+let lemma_InDomRestrict #key #value m ks k = ()
+let lemma_ContainsDom #key #value m k      = ()
+let lemma_UpdDomain #key #value m k v      = ()
 
 abstract type equal (#key:eqtype) (#value:Type) (m1:t key value) (m2:t key value) =
-    feq m1.mappings m2.mappings /\ Set.equal m1.domain m2.domain
+    feq m1.mappings m2.mappings /\ equal m1.domain m2.domain
 
 
-abstract val lemma_equal_intro: m1:t 'key 'value -> m2:t 'key 'value ->
-                       Lemma (requires (forall k. sel m1 k = sel m2 k /\
+abstract val lemma_equal_intro: #key:eqtype -> #value:Type -> m1:t key value -> m2:t key value ->
+                       Lemma (requires (forall k. sel m1 k == sel m2 k /\
                                                   contains m1 k = contains m2 k))
                        (ensures (equal m1 m2))
                        [SMTPatT (equal m1 m2)]
 
-abstract val lemma_equal_elim: m1:t 'key 'value -> m2:t 'key 'value ->
-                      Lemma (requires (equal m1 m2)) (ensures  (m1 = m2))
+abstract val lemma_equal_elim: #key:eqtype -> #value:Type -> m1:t key value -> m2:t key value ->
+                      Lemma (requires (equal m1 m2)) (ensures  (m1 == m2))
                       [SMTPatT (equal m1 m2)]
 
-abstract val lemma_equal_refl: m1:t 'key 'value -> m2:t 'key 'value ->
-                      Lemma  (requires (m1 = m2)) (ensures  (equal m1 m2))
+abstract val lemma_equal_refl: #key:eqtype -> #value:Type -> m1:t key value -> m2:t key value ->
+                      Lemma  (requires (m1 == m2)) (ensures  (equal m1 m2))
 		      [SMTPatT (equal m1 m2)]
 
 
-let lemma_equal_intro m1 m2 = ()
-let lemma_equal_elim m1 m2  = ()
-let lemma_equal_refl m1 m2  = ()
+let lemma_equal_intro #key #value m1 m2 = ()
+let lemma_equal_elim #key #value m1 m2  = ()
+let lemma_equal_refl #key #value m1 m2  = ()
 
 let const_on (#key:eqtype) (#value:Type) (dom:set key) (v:value) = restrict dom (const v)
 
